Hs.lean
@@ -1,6 +1,5 @@
 import Hs.HsTerm
 import Hs.HsJudgment
 import Hs.Algorithm
--- import Hs.CompileJ
-import Hs.Metatheory.Preservation2
+import Hs.Metatheory.Preservation3
 import Hs.Example
