Hs/Metatheory/Preservation3.lean
@@ -1,0 +1,129 @@
+import Hs.Algorithm
+import Hs.Metatheory.Uniqueness
+import Hs.Metatheory.Weaken
+import Hs.Metatheory.WeakenCompile
+import Hs.Metatheory.Substitution
+import Hs.Metatheory.SubstitutionCompile
+import Hs.Metatheory.TypeMatchCompile
+import Hs.Metatheory.Preservation1
+import Hs.Metatheory.Preservation2
+import SystemFD.Algorithm.Soundness2
+
+---------------------------------------------
+-- Contexts
+--------------------------------------------
+theorem compile_preserves_ctx_shape Γ :
+  ⊢s Γ -> (Η : HsCtx Γ) ->
+  compile_ctx Η = .some Γ' ->
+  (Γ d@ x).get_type = .some T ->
+  (j : Γ ⊢κ T : `□) ->
+  compile .kind Γ ⟨(T, `□), j⟩ = .some T' ->
+  (Γ' d@ x).get_type = .some T'
+ := by
+intro wf h cc gt j ck;
+induction h generalizing Γ';
+case _ => cases gt
+case _ Γ h ih =>
+  cases wf; case _ wf =>
+  unfold compile_ctx at cc; simp at cc;
+  rw[Option.bind_eq_some] at cc;
+  cases cc; case _ wΓ cc =>
+  cases cc; case _ cc cc1 =>
+  rw[Option.bind_eq_some] at cc1;
+  cases cc1; case _ u cc1 =>
+  cases cc1; case _ cc1 e =>
+  cases e;
+  have ih' := @ih wΓ wf cc
+  sorry
+case _ => sorry
+case _ => sorry
+case _ => sorry
+case _ => sorry
+case _ => sorry
+case _ => sorry
+
+
+theorem compile_preserves_wf Γ :
+  ⊢s Γ -> (Η : HsCtx Γ) -> compile_ctx Η = .some Γ' -> ⊢ Γ' := by
+intro wf h cc;
+induction h generalizing Γ';
+case _ =>
+  unfold compile_ctx at cc; cases cc;
+  apply Judgment.wfnil;
+case _ ih =>
+  cases wf; case _ wf =>
+  unfold compile_ctx at cc; simp at cc;
+  rw[Option.bind_eq_some] at cc;
+  cases cc; case _ w cc =>
+  cases cc; case _ cc cc1 =>
+  rw[Option.bind_eq_some] at cc1;
+  cases cc1; case _ w1 cc1 =>
+  cases cc1; case _ cc1 cc2 =>
+  cases cc2;
+  apply Judgment.wfempty;
+  apply wf_ctx_sound cc1;
+case _ j ih =>
+  cases wf; case _ wf jk =>
+  unfold compile_ctx at cc; simp at cc;
+  rw[Option.bind_eq_some] at cc;
+  cases cc; case _ w cc =>
+  cases cc; case _ cc cc1 =>
+  rw[Option.bind_eq_some] at cc1;
+  cases cc1; case _ w1 cc1 =>
+  cases cc1; case _ cc1 cc2 =>
+  rw[Option.bind_eq_some] at cc2;
+  cases cc2; case _ w2 cc2 =>
+  cases cc2; case _ cc2 cc3 =>
+  cases cc3; cases w1;
+  apply Judgment.wfkind;
+  apply compile_preserves_kinds _ j cc2;
+  case _ => apply @ih w wf cc
+  apply @ih w wf cc
+case _ j ih =>
+  cases wf; case _ wf jk =>
+  unfold compile_ctx at cc; simp at cc;
+  rw[Option.bind_eq_some] at cc;
+  cases cc; case _ w cc =>
+  cases cc; case _ cc cc1 =>
+  rw[Option.bind_eq_some] at cc1;
+  cases cc1; case _ w1 cc1 =>
+  cases cc1; case _ cc1 cc2 =>
+  rw[Option.bind_eq_some] at cc2;
+  cases cc2; case _ w2 cc2 =>
+  cases cc2; case _ cc2 cc3 =>
+  cases cc3; cases w1;
+  apply Judgment.wfdatatype;
+  apply compile_preserves_kinds _ j cc2;
+  case _ => apply @ih w wf cc
+  apply @ih w wf cc
+case _ Γ τ a j ih =>
+  cases wf; case _ wf jk =>
+  unfold compile_ctx at cc; simp at cc;
+  rw[Option.bind_eq_some] at cc;
+  cases cc; case _ Γ' cc =>
+  cases cc; case _ cc cc1 =>
+  rw[Option.bind_eq_some] at cc1;
+  cases cc1; case _ w1 cc1 =>
+  cases cc1; case _ cc1 cc2 =>
+  rw[Option.bind_eq_some] at cc2;
+  cases cc2; case _ τ' cc2 =>
+  cases cc2; case _ cc2 cc3 =>
+  cases cc3; cases w1;
+  have lem := @ih Γ' wf cc
+  have lemAx : Γ ⊢κ `★ : `□ := by apply HsJudgment.ax (hs_judgment_ctx_wf .type jk)
+  have lemK : compile_kind Γ `★ `□ lemAx = .some ★ := by unfold compile_kind; cases lemAx; simp
+  apply Judgment.wftype;
+  apply compile_preserves_types _ lem _ lemAx lemK j cc2;
+  case _ =>
+    simp;
+    intros Γ Γ' x T T' wf gt j ck;
+    unfold compile at ck; simp at ck; sorry
+  case _ => intros; sorry
+  assumption
+
+case _ ih =>
+  cases wf; case _ wf j vhv =>
+  unfold compile_ctx at cc; simp at cc;
+  sorry
+case _ => sorry
+case _ => sorry
