Hs/Metatheory/TypeMatchCompile.lean
@@ -7,40 +7,111 @@ import Hs.Metatheory.SubstitutionCompile
 import Hs.Metatheory.Preservation1
 import SystemFD.Algorithm.Soundness2
 
+theorem compile_preserves_type_neutral_form :
+  ⊢ Γ' ->
+  (j : Γ ⊢τ t : k) ->
+  compile_type Γ t k j = .some t' ->
+  t.neutral_form = .some (h, sp) ->
+  ∃ h' sp', t'.neutral_form = .some (h', sp') := by
+intro wf j ct tnf;
+induction Γ, t, k, j using compile_type.induct generalizing Γ' t' h sp
+case _ x _ _ _ _ =>
+  unfold compile_type at ct; simp at ct;
+  rw[Option.bind_eq_some] at ct;
+  cases ct; case _ k ct =>
+  cases ct; case _ ct e =>
+  cases e; exists x; exists []
+case _ a _ _ _ _ ih _ =>
+  unfold compile_type at ct; simp at ct;
+  rw[Option.bind_eq_some] at ct;
+  cases ct; case _ A' ct =>
+  cases ct; case _ ct ct1 =>
+  rw[Option.bind_eq_some] at ct1;
+  cases ct1; case _ B' ct1 =>
+  cases ct1; case _ ct1 ct2 =>
+  rw[Option.bind_eq_some] at ct2;
+  cases ct2; case _ f' ct2 =>
+  cases ct2; case _ ct2 ct3 =>
+  rw[Option.bind_eq_some] at ct3;
+  cases ct3; case _ a' ct3 =>
+  cases ct3; case _ ct3 e =>
+  cases e
+  unfold HsTerm.neutral_form at tnf; simp at tnf;
+  rw[Option.bind_eq_some] at tnf;
+  cases tnf; case _ nf tnf =>
+  cases tnf; case _ fnf e =>
+  cases e;
+  have ih' := @ih Γ' f' nf.1 nf.snd wf ct2 fnf
+  cases ih'; case _ h' ih' =>
+  cases ih'; case _ sp' ih' =>
+  exists h'; exists (sp' ++ [( SpineVariant.kind, a') ]);
+  unfold Term.neutral_form; simp;
+  rw[Option.bind_eq_some];
+  exists (h', sp');
+all_goals (cases tnf)
 
-theorem compile_type_match :
- -- (∀ Γ (h1 h2 : ⊢s Γ), h1 = h2) ->
- (∀ v, CompileCtxPred v) ->
- ⊢ Γ' ->
- (jA : Γ ⊢τ A : `★) ->
- compile_type Γ A `★ jA = .some A' ->
- (jA : Γ ⊢τ R : `★) ->
- compile_type Γ R `★ jR = .some R' ->
- StableHsTypeMatch Γ A R -> StableTypeMatch Γ' A' R' := by sorry
+-- theorem compile_preserves_term_neutral_form :
+--   ⊢ Γ' ->
+--   (j1 : Γ ⊢τ A : `★) ->
+--   (j2 : Γ ⊢t t : A) ->
+--   compile_term Γ t A j2 = .some t' ->
+--   t.neutral_form = .some (h, sp) ->
+--   ∃ h' sp', t'.neutral_form = .some (h', sp') := by
+-- intro wf h1 ht ct tnf;
+-- induction Γ, t, A, ht using compile_term.induct generalizing Γ' t' h sp <;> simp at *
+-- all_goals try (cases tnf)
+-- case _ x _ _ _ e1 e2 =>
+--   cases e1; cases e2
+--   exists x; exists [];
+--   unfold compile_term at ct; cases ct; rfl
+-- case _ Γ t1 A B t2 j1 j2 j3 j4 ih _ =>
+--   rw[Option.bind_eq_some] at tnf;
+--   cases tnf; case _ nf tnf =>
+--   cases tnf; case _ tnf e =>
+--   cases e;
+--   unfold compile_term at ct; simp at ct;
+--   rw[Option.bind_eq_some] at ct;
+--   cases ct; case _ AB' ct =>
+--   cases ct; case _ ct ct1 =>
+--   rw[Option.bind_eq_some] at ct1;
+--   cases ct1; case _ A' ct1 =>
+--   cases ct1; case _ ct1 ct2 =>
+--   rw[Option.bind_eq_some] at ct2;
+--   cases ct2; case _ B' ct2 =>
+--   cases ct2; case _ ct2 ct3 =>
+--   rw[Option.bind_eq_some] at ct3;
+--   cases ct3; case _ t1' ct3 =>
+--   cases ct3; case _ ct3 ct4 =>
+--   rw[Option.bind_eq_some] at ct4;
+--   cases ct4; case _ t2' ct4 =>
+--   cases ct4; case _ ct4 e =>
+--   cases e;
+--   have ih' := @ih Γ' t1' nf.1 nf.2 wf (extract_typing j1) ct3 tnf
+--   cases ih'; case _ h' ih' =>
+--   cases ih'; case _ sp' ih' =>
+--   exists h'; exists (sp' ++ [(.term, t2')]);
+--   simp; rw[Option.bind_eq_some];
+--   exists (h', sp');
+-- case _ Γ t A τ e j1 j2 j3 j4 j5 ih =>
+--   unfold compile_term at ct; simp at ct
+--   rw[Option.bind_eq_some] at ct;
+--   cases ct; case _ Aτ' ct =>
+--   cases ct; case _ ct ct1 =>
+--   rw[Option.bind_eq_some] at ct1;
+--   cases ct1; case _ A' ct1 =>
+--   cases ct1; case _ ct1 ct2 =>
+--   rw[Option.bind_eq_some] at ct2;
+--   cases ct2; case _ t' ct2 =>
+--   cases ct2; case _ ct2 ct3 =>
+--   rw[Option.bind_eq_some] at ct3;
+--   cases ct3; case _ a' ct3 =>
+--   cases ct3; case _ ct3 e =>
+--   cases e;
 
-
-theorem compile_stable_match :
- -- (∀ Γ (h1 h2 : ⊢s Γ), h1 = h2) ->
- (∀ v, CompileCtxPred v) ->
- ⊢ Γ' ->
- (jA : Γ ⊢τ A : `★) ->
- compile_type Γ A `★ jA = .some A' ->
- (jR : Γ ⊢τ R : `★) ->
- compile_type Γ R `★ jR = .some R' ->
- StableHsTypeMatch Γ A R -> StableTypeMatch Γ' A' R' := by sorry
-
-
-theorem compile_prefix_match :
- -- (∀ Γ (h1 h2 : ⊢s Γ), h1 = h2) ->
- (∀ v, CompileCtxPred v) ->
- ⊢ Γ' ->
- (jA : Γ ⊢τ A : `★) ->
- compile_type Γ A `★ jA = .some A' ->
- (jR : Γ ⊢τ R : `★) ->
- compile_type Γ R `★ jR = .some R' ->
- (jT : Γ ⊢τ T : `★) ->
- compile_type Γ T `★ jT = .some T' ->
- PrefixHsTypeMatch Γ A R T -> PrefixTypeMatch Γ' A' R' T' := by sorry
+--   sorry
+-- case _ => sorry
+-- case _ => sorry
+-- case _ => sorry
 
 theorem compile_preserves_vhv_types test σtest :
  (∀ v, CompileCtxPred v) ->
@@ -58,3 +129,89 @@ theorem compile_preserves_vhv_terms test σtest :
  compile_term Γ T τ jT = .some T' ->
  HsValidHeadVariable T test ->
  ValidHeadVariable T' σtest := by sorry
+
+theorem compile_stable_match :
+ (∀ Γ (h1 h2 : ⊢s Γ), h1 = h2) ->
+ (∀ v, CompileCtxPred v) ->
+ ⊢ Γ' ->
+ (jA : Γ ⊢τ A : `★) ->
+ compile_type Γ A `★ jA = .some A' ->
+ (jR : Γ ⊢τ R : `★) ->
+ compile_type Γ R `★ jR = .some R' ->
+ StableHsTypeMatch Γ A R -> StableTypeMatch Γ' A' R' := by
+intro h cc wf jA cA jR cR stm;
+induction stm generalizing Γ' A' R';
+case _ R Γ vhv =>
+  have u := compile_type_uniqueness h jA jR cA cR; cases u
+  apply StableTypeMatch.refl;
+  apply compile_preserves_vhv_types Γ.is_stable Γ'.is_stable cc wf jR cR vhv;
+case _ R Γ B A vhv stm ih =>
+  have lem := compile_preserves_type_shape_arrow jA cA;
+  cases lem; case _ A' lem =>
+  cases lem; case _ B' lem =>
+  cases lem; case _ jA' lem =>
+  cases lem; case _ jB' lem =>
+  cases lem; case _ e lem =>
+  subst e
+  cases lem; case _ cA' cB' =>
+  apply StableTypeMatch.arrow;
+  apply compile_preserves_vhv_types Γ.is_stable Γ'.is_stable cc wf jR cR vhv
+  have lem := weaken_compile_type jR cR (hs_weaken_empty_type jR)
+  apply @ih (.empty :: Γ') B' ([S]R') _ jB' cB' (hs_weaken_empty_type jR) lem
+  case _ => apply Judgment.wfempty wf
+
+case _ R Γ B A vhv stm ih =>
+  have lem := compile_preserves_type_shape_farrow jA cA;
+  cases lem; case _ A' lem =>
+  cases lem; case _ B' lem =>
+  cases lem; case _ jA' lem =>
+  cases lem; case _ jB' lem =>
+  cases lem; case _ e lem =>
+  subst e
+  cases lem; case _ cA' cB' =>
+  apply StableTypeMatch.arrow;
+  apply compile_preserves_vhv_types Γ.is_stable Γ'.is_stable cc wf jR cR vhv
+  have lem := weaken_compile_type jR cR (hs_weaken_empty_type jR)
+  apply @ih (.empty :: Γ') B' ([S]R') _ jB' cB' (hs_weaken_empty_type jR) lem
+  case _ => apply Judgment.wfempty wf
+
+case _ R Γ A B vhv stm ih =>
+  have lem := compile_preserves_type_shape_all jA cA;
+  cases lem; case _ A' lem =>
+  cases lem; case _ B' e =>
+  subst e
+  case _ cA' cB' =>
+  apply StableTypeMatch.all;
+  apply compile_preserves_vhv_types Γ.is_stable Γ'.is_stable cc wf jR cR vhv
+  unfold compile_type at cA; cases jA; simp at cA; case _ jA jB =>
+  rw[Option.bind_eq_some] at cA;
+  cases cA; case _ A' cA =>
+  cases cA; case _ cA cB =>
+  rw[Option.bind_eq_some] at cB;
+  cases cB; case _ B' cB =>
+  cases cB; case _ cB e =>
+  cases e;
+  have lem := weaken_compile_type jR cR (hs_weaken_kind_type jA jR)
+  apply @ih (.kind A' :: Γ') B' ([S]R') _ jB cB (hs_weaken_kind_type jA jR) lem
+  apply Judgment.wfkind; apply compile_preserves_kinds wf jA cA; apply wf
+
+theorem compile_prefix_match :
+ (∀ Γ (h1 h2 : ⊢s Γ), h1 = h2) ->
+ (∀ v, CompileCtxPred v) ->
+ ⊢ Γ' ->
+ (jA : Γ ⊢τ A : `★) ->
+ compile_type Γ A `★ jA = .some A' ->
+ (jR : Γ ⊢τ R : `★) ->
+ compile_type Γ R `★ jR = .some R' ->
+ (jT : Γ ⊢τ T : `★) ->
+ compile_type Γ T `★ jT = .some T' ->
+ PrefixHsTypeMatch Γ A R T -> PrefixTypeMatch Γ' A' R' T' := by
+intro h cc wf jA cA jR cR jT cT ptm;
+induction ptm generalizing Γ' A' R' T'
+case _ =>
+
+  sorry
+case _ =>
+ sorry
+case _ =>
+ sorry
